Problem fill for LetBinder and extra lemmas composition for LetPattern

2016/Ext_Structures.thy
@@ -2,6 +2,7 @@
 theory Ext_Structures
 imports
    Main
+   List_extra
   "~~/src/HOL/List"
   "~~/src/HOL/Eisbach/Eisbach"
   "~~/src/HOL/Eisbach/Eisbach_Tools"
@@ -13,15 +14,16 @@ section{*Pair, Tuples and Records*}
 
 text{* In this section,we extend our current lambda calculus with extended structures (pairs, tuples, records)*}
 
-
-
 datatype ltype =
   Bool |
   T (num:nat) |
   Unit |
   Prod ltype ltype (infix "|\<times>|" 225)|
   Fun (domain: ltype) (codomain: ltype) (infixr "\<rightarrow>" 225)|
-  TupleT "ltype list" ( "\<lparr>_\<rparr>" [150]225)
+  TupleT "ltype list" ( "\<lparr>_\<rparr>" [150]225) |
+  RecordT "string list" "ltype list" ( "\<lparr>_|:|_\<rparr>" [150,150] 225)
+
+datatype Lpattern = V nat | RCD "string list" "Lpattern list"
 
 datatype lterm =
   LTrue |
@@ -38,7 +40,14 @@ datatype lterm =
   Proj1 lterm ("\<pi>1/ _" [100] 250) |
   Proj2 lterm ("\<pi>2/ _" [100] 250) |
   Tuple "lterm list" |
-  ProjT nat lterm ("\<Pi>/ _/ (_)" [100,150] 250)
+  ProjT nat lterm ("\<Pi>/ _/ (_)" [100,150] 250) |
+  Record "string list" "lterm list" |
+  ProjR string lterm |
+  Pattern Lpattern ("<|_|>" [100] 250)|
+  LetP Lpattern lterm lterm ("Let/ pattern/ (_)/ :=/ (_)/ in/ (_)"[100,120,150]250)
+  
+abbreviation Record1 :: "(string\<times>lterm) list \<Rightarrow> lterm" where
+"Record1 L \<equiv> Record (map fst L) (map snd L)"
 
 primrec shift_L :: "int \<Rightarrow> nat \<Rightarrow> lterm \<Rightarrow> lterm" where
   "shift_L d c LTrue = LTrue" |
@@ -57,8 +66,12 @@ primrec shift_L :: "int \<Rightarrow> nat \<Rightarrow> lterm \<Rightarrow> lter
   "shift_L d c (\<lbrace>t1,t2\<rbrace>) = \<lbrace> shift_L d c t1 , shift_L d c t2 \<rbrace>" |
   "shift_L d c (\<pi>1 t) = \<pi>1 (shift_L d c t)" |
   "shift_L d c (\<pi>2 t) = \<pi>2 (shift_L d c t)" |
-  "shift_L d c (Tuple L) = Tuple (map (\<lambda>t. shift_L d c t) L)" |
-  "shift_L d c (\<Pi> i t) = \<Pi> i (shift_L d c t)"
+  "shift_L d c (Tuple L) = Tuple (map (shift_L d c) L)" |
+  "shift_L d c (\<Pi> i t)   = \<Pi> i (shift_L d c t)" |
+  "shift_L d c (Record L LT)  = Record L (map (shift_L d c) LT)" |
+  "shift_L d c (ProjR l t) = ProjR l (shift_L d c t)" |
+  "shift_L d c (Pattern p) = Pattern p" |
+  "shift_L d c (Let pattern p := t1 in t2) = (Let pattern p := (shift_L d c t1) in (shift_L d c t2))"
 
 primrec subst_L :: "nat \<Rightarrow> lterm \<Rightarrow> lterm \<Rightarrow> lterm" where
   "subst_L j s LTrue = LTrue" |
@@ -76,8 +89,12 @@ primrec subst_L :: "nat \<Rightarrow> lterm \<Rightarrow> lterm \<Rightarrow> lt
   "subst_L j s (\<lbrace>t1,t2\<rbrace>) = \<lbrace>subst_L j s t1, subst_L j s t2\<rbrace>" |
   "subst_L j s (\<pi>1 t) = \<pi>1 (subst_L j s t)" |
   "subst_L j s (\<pi>2 t) = \<pi>2 (subst_L j s t)" |
-  "susbt_L j s (Tuple L) = Tuple (map (\<lambda>t. subst_L j s t) L)" |
-  "subst_L j s (\<Pi> i t) = \<Pi> i (subst_L j s t)"
+  "subst_L j s (\<Pi> i t) = \<Pi> i (subst_L j s t)" |
+  "subst_L j s (Tuple L) = Tuple (map (subst_L j s) L)" |
+  "subst_L j s (Record L LT) = Record L (map (subst_L j s) LT)" |
+  "subst_L j s (ProjR l t) = ProjR l (subst_L j s t)" |
+  "subst_L j s (Pattern p) = Pattern p" |
+  "subst_L j s (Let pattern p := t1 in t2) = (Let pattern p := (subst_L j s t1) in (subst_L j s t2))"
 
 inductive is_value_L :: "lterm \<Rightarrow> bool" where
   "is_value_L LTrue" |
@@ -85,11 +102,8 @@ inductive is_value_L :: "lterm \<Rightarrow> bool" where
   "is_value_L (LAbs T' t)" |
   "is_value_L unit" |
   "is_value_L v1 \<Longrightarrow> is_value_L v2 \<Longrightarrow> is_value_L (\<lbrace>v1,v2\<rbrace>)" |
-  "(\<And>i.0\<le>i \<Longrightarrow> i<length L \<Longrightarrow> is_value_L (L!i)) \<Longrightarrow> is_value_L (Tuple L)"
-
-fun list_iter ::"('a\<Rightarrow>'b \<Rightarrow> 'b) \<Rightarrow> 'b \<Rightarrow> 'a list \<Rightarrow> 'b" where
-"list_iter f r [] = r" |
-"list_iter f r (a#xs) = f a (list_iter f r xs)"
+  "(\<And>i.0\<le>i \<Longrightarrow> i<length L \<Longrightarrow> is_value_L (L!i)) \<Longrightarrow> is_value_L (Tuple L)" |
+  "(\<And>i.0\<le>i \<Longrightarrow> i<length LT \<Longrightarrow> is_value_L (LT!i)) \<Longrightarrow> is_value_L (Record L LT)"
 
 primrec FV :: "lterm \<Rightarrow> nat set" where
   "FV LTrue = {}" |
@@ -107,16 +121,75 @@ primrec FV :: "lterm \<Rightarrow> nat set" where
   "FV (\<pi>1 t) =  FV t" |
   "FV (\<pi>2 t) =  FV t" |
   "FV (Tuple L) = list_iter (\<lambda>x r. x \<union> r) {} (map FV L) "|
-  "FV (\<Pi> i t) = FV t"
+  "FV (\<Pi> i t) = FV t" |
+  "FV (Record L LT) = list_iter (\<lambda>x r. x \<union> r) {} (map FV LT) "|
+  "FV (ProjR l t) = FV t" |
+  "FV (Pattern p) = {}" |
+  "FV (Let pattern p := t1 in t2) = FV t1 \<union> FV t2"
 
-fun replace ::"nat \<Rightarrow> 'a \<Rightarrow> 'a list \<Rightarrow> 'a list" where
-"replace n x xs = 
-  (if length xs \<le> n then xs 
-    else (take n xs) @ [x] @ (drop (Suc n) xs))"
 
-lemma replace_inv_length[simp]:
-  "length (replace n x S) = length S"  
-by(induction S arbitrary: x n, auto)
+
+text{*
+    We implement pattern matching and replacing with the following function and definition:
+    
+    \begin{itemize}
+      \item a \textbf{pattern context} 
+      \item a \textbf{pattern substitution} is a list of pairs (pattern var index, lterm)
+      \item \textbf{fill}, which will fill the patterns in a ltern with a lterm (based on a pattern substitution)
+      \item \textbf{Lmatch} is a predicate on a pattern, a value and a pattern substitution indicating 
+              if the pattern substitution associates the given pattern's variables to the corresponding part(s) of the
+              given value
+    \end{itemize}
+*}
+
+fun p_instantiate::"(nat \<times> lterm) list \<Rightarrow> Lpattern \<Rightarrow> lterm" where
+"p_instantiate \<Delta> (V k) = (case (find (\<lambda>p. fst p = k) \<Delta>) of None \<Rightarrow> <|V k|> | Some p \<Rightarrow> snd p)"|
+"p_instantiate \<Delta> (RCD L PL) = Record L (map (p_instantiate \<Delta>) PL)"
+
+fun fill::"(nat \<times> lterm) list \<Rightarrow> lterm \<Rightarrow> lterm" where
+"fill \<Delta> (Pattern p)                 = p_instantiate \<Delta> p" |
+"fill \<Delta> (LIf c t1 t2)               = LIf (fill \<Delta> c) (fill \<Delta> t1) (fill \<Delta> t2)" |
+"fill \<Delta> (LAbs A t1)                 = LAbs A (fill \<Delta> t1)" |
+"fill \<Delta> (LApp t1 t2)                = LApp (fill \<Delta> t1) (fill \<Delta> t2)" |
+"fill \<Delta> (Seq t1 t2)                 =  Seq (fill \<Delta> t1) (fill \<Delta> t2)" |
+"fill \<Delta> (t1 as A)                   = (fill \<Delta> t1) as A" |
+"fill \<Delta> (Let var x := t1 in t2)     = (Let var x := (fill \<Delta> t1) in (fill \<Delta> t2))" |
+"fill \<Delta> (\<lbrace>t1,t2\<rbrace>)                   = \<lbrace>(fill \<Delta> t1), (fill \<Delta> t2)\<rbrace>" |
+"fill \<Delta> (Tuple L)                   = Tuple (map (fill \<Delta>) L)" |
+"fill \<Delta> (Record L LT)               = Record L (map (fill \<Delta>) LT)" |
+"fill \<Delta> (\<pi>1 t)                      = \<pi>1 (fill \<Delta> t)" |
+"fill \<Delta> (\<pi>2 t)                      = \<pi>2 (fill \<Delta> t)" |
+"fill \<Delta> (\<Pi> i t)                     = \<Pi> i (fill \<Delta> t)" |
+"fill \<Delta> (ProjR l t)                 = ProjR l (fill \<Delta> t)" |
+"fill \<Delta> (Let pattern p := t1 in t2) = (Let pattern p := (fill \<Delta> t1) in (fill \<Delta> t2))" |
+"fill \<Delta> t = t"
+
+inductive Lmatch ::"Lpattern \<Rightarrow> lterm \<Rightarrow> (nat\<times>lterm) list \<Rightarrow> bool" where
+  M_Var:
+    "is_value_L v \<Longrightarrow> Lmatch (V n) v [(n,v)]" |
+  M_RCD:
+    "distinct L \<Longrightarrow> length L = length LT \<Longrightarrow> length F = length PL \<Longrightarrow> length PL = length LT 
+    \<Longrightarrow> is_value_L (Record L LT) \<Longrightarrow> (\<And>i. 0\<le>i \<Longrightarrow> i<length PL \<Longrightarrow> Lmatch (PL!i) (LT!i) (F!i))
+    \<Longrightarrow> Lmatch (RCD L PL) (Record L LT) (list_iter (\<lambda>g r. g @ r) [] F)"
+
+text{*
+      We want to restrict the considered pattern matching and filling to coherent cases, which are
+      the cases when a pattern variable can only appear once in a given pattern.\\
+
+      Furthermore, the same coherence principle is valid for the pattern context. A pattern variable can only 
+      have on type at a time
+*}
+
+primrec Pvars :: "Lpattern \<Rightarrow> nat list" where
+"Pvars (V n) = [n]" |
+"Pvars (RCD L PL) = (list_iter (\<lambda>x r. x @ r) [] (map Pvars PL))"
+
+
+abbreviation coherent_Subst :: "(nat\<times>ltype) list \<Rightarrow> bool" where
+"coherent_Subst \<Delta> \<equiv> distinct(fst_extract \<Delta>)"
+
+abbreviation coherent ::"Lpattern \<Rightarrow> bool" where
+"coherent p \<equiv> distinct (Pvars p)"
 
 
 inductive eval1_L :: "lterm \<Rightarrow> lterm \<Rightarrow> bool" where
@@ -167,15 +240,30 @@ inductive eval1_L :: "lterm \<Rightarrow> lterm \<Rightarrow> bool" where
     "eval1_L t1 t1' \<Longrightarrow> eval1_L (\<lbrace>t1,t2\<rbrace>) (\<lbrace>t1',t2\<rbrace>)" |
   eval1_L_Pair2:
     "is_value_L v1 \<Longrightarrow> eval1_L t2 t2' \<Longrightarrow> eval1_L (\<lbrace>v1,t2\<rbrace>) (\<lbrace>v1,t2'\<rbrace>)" |
+ -- "Rules relating to evaluation of tuples"
   eval1_L_ProjTuple:
     "1\<le>i \<Longrightarrow> i\<le>length L \<Longrightarrow> is_value_L (Tuple L) \<Longrightarrow> eval1_L (\<Pi> i (Tuple L)) (L ! (i-1))" |
   eval1_L_Proj:
     "eval1_L t1 t1' \<Longrightarrow> eval1_L (\<Pi> i t1) (\<Pi> i t1')" |
   eval1_L_Tuple:
-    " 1\<le>j\<Longrightarrow> i\<le>length L \<Longrightarrow> is_value_L (Tuple (take (j-1) L)) \<Longrightarrow> 
-      eval1_L (L ! (j-1)) (t') \<Longrightarrow> eval1_L (Tuple L) (Tuple (replace (j-1) t' L))"
-    
+    " 1\<le>j\<Longrightarrow> j\<le>length L \<Longrightarrow> is_value_L (Tuple (take (j-1) L)) \<Longrightarrow> 
+      eval1_L (L ! (j-1)) (t') \<Longrightarrow> eval1_L (Tuple L) (Tuple (replace (j-1) t' L))" |
+ -- "Rules relating to evaluation of records"
+  eval1_L_ProjRCD:
+    "l \<in> set L \<Longrightarrow> is_value_L (Record L LT) \<Longrightarrow> eval1_L (ProjR l (Record L LT)) (LT ! (index L l))" |
+  eval1_L_ProjR:
+    "eval1_L t1 t1' \<Longrightarrow> eval1_L (ProjR i t1) (ProjR i t1')" |
+  eval1_L_RCD:
+    " l\<in>set L \<Longrightarrow> index L l = m \<Longrightarrow> is_value_L (Record (take m L) (take m LT)) \<Longrightarrow> 
+      eval1_L (LT ! m) (t') \<Longrightarrow> eval1_L (Record L LT) (Record L (replace m t' LT))" |   
+ -- "Rules relating to evaluation of pattern matching"
+  eval1_L_LetPV:
+    "coherent p \<Longrightarrow> is_value_L v1 \<Longrightarrow> Lmatch p v1 \<sigma> \<Longrightarrow> eval1_L (Let pattern p := v1 in t2) (fill \<sigma> t2)" |
+  eval1_L_LetP:
+    "eval1_L t1 t1' \<Longrightarrow> eval1_L (Let pattern p := t1 in t2) (Let pattern p := t1' in t2)"
+
 type_synonym lcontext = "ltype list"
+type_synonym pcontext = "(nat\<times>ltype) list"
 
 notation Nil ("\<emptyset>")
 abbreviation cons :: "lcontext \<Rightarrow> ltype \<Rightarrow> lcontext" (infixl "|,|" 200) where
@@ -187,75 +275,151 @@ text{*  For the typing rule of letbinder, we require to replace the type
         of the variable by the expected type 
     *}
 
-
-inductive has_type_L :: "lcontext \<Rightarrow> lterm \<Rightarrow> ltype \<Rightarrow> bool" ("((_)/ \<turnstile> (_)/ |:| (_))" [150, 150, 150] 150) where
+inductive has_type_L :: "pcontext \<Rightarrow> lcontext \<Rightarrow> lterm \<Rightarrow> ltype \<Rightarrow> bool" ("((_)|;|(_)/ \<turnstile> (_)/ |:| (_))" [150, 150, 150, 150] 150) where
   -- "Rules relating to the type of Booleans"
   has_type_LTrue:
-    "\<Gamma> \<turnstile> LTrue |:| Bool" |
+    "\<Delta> |;| \<Gamma> \<turnstile> LTrue |:| Bool" |
   has_type_LFalse:
-    "\<Gamma> \<turnstile> LFalse |:| Bool" |
+    "\<Delta> |;| \<Gamma> \<turnstile> LFalse |:| Bool" |
   has_type_LIf:
-    "\<Gamma> \<turnstile> t1 |:| Bool \<Longrightarrow> \<Gamma> \<turnstile> t2 |:| T' \<Longrightarrow> \<Gamma> \<turnstile> t3 |:| T' \<Longrightarrow> \<Gamma> \<turnstile> (LIf t1 t2 t3) |:| T'" |
+    "\<Delta> |;| \<Gamma> \<turnstile> t1 |:| Bool \<Longrightarrow> \<Delta> |;| \<Gamma> \<turnstile> t2 |:| T' \<Longrightarrow> \<Delta> |;| \<Gamma> \<turnstile> t3 |:| T' \<Longrightarrow> \<Delta> |;| \<Gamma> \<turnstile> (LIf t1 t2 t3) |:| T'" |
 
   -- \<open>Rules relating to the type of the constructs of the $\lambda$-calculus\<close>
   has_type_LVar:
-    "(x, T') |\<in>| \<Gamma> \<Longrightarrow> \<Gamma> \<turnstile> (LVar x) |:| (T')" |
+    "(x, T') |\<in>| \<Gamma> \<Longrightarrow> \<Delta> |;| \<Gamma> \<turnstile> (LVar x) |:| (T')" |
   has_type_LAbs:
-    "(\<Gamma> |,| T1) \<turnstile> t2 |:| T2 \<Longrightarrow> \<Gamma> \<turnstile> (LAbs T1 t2) |:| (T1 \<rightarrow> T2)" |
+    "\<Delta> |;|(\<Gamma> |,| T1) \<turnstile> t2 |:| T2 \<Longrightarrow> \<Delta> |;| \<Gamma> \<turnstile> (LAbs T1 t2) |:| (T1 \<rightarrow> T2)" |
   has_type_LApp:
-    "\<Gamma> \<turnstile> t1 |:| (T11 \<rightarrow> T12) \<Longrightarrow> \<Gamma> \<turnstile> t2 |:| T11 \<Longrightarrow> \<Gamma> \<turnstile> (LApp t1 t2) |:| T12" |  
+    "\<Delta> |;| \<Gamma> \<turnstile> t1 |:| (T11 \<rightarrow> T12) \<Longrightarrow> \<Delta> |;| \<Gamma> \<turnstile> t2 |:| T11 \<Longrightarrow> \<Delta> |;| \<Gamma> \<turnstile> (LApp t1 t2) |:| T12" |  
   has_type_LUnit:
-    "\<Gamma> \<turnstile> unit |:| Unit " |  
+    "\<Delta> |;| \<Gamma> \<turnstile> unit |:| Unit " |  
   has_type_LSeq:
-    "\<Gamma> \<turnstile> t1 |:| Unit \<Longrightarrow> \<Gamma> \<turnstile> t2 |:| A \<Longrightarrow> \<Gamma> \<turnstile> (Seq t1 t2) |:| A" |
+    "\<Delta> |;| \<Gamma> \<turnstile> t1 |:| Unit \<Longrightarrow> \<Delta> |;| \<Gamma> \<turnstile> t2 |:| A \<Longrightarrow> \<Delta> |;| \<Gamma> \<turnstile> (Seq t1 t2) |:| A" |
   has_type_LAscribe:
-    "\<Gamma> \<turnstile> t1 |:| A \<Longrightarrow> \<Gamma> \<turnstile> t1 as A |:| A" |
+    "\<Delta> |;| \<Gamma> \<turnstile> t1 |:| A \<Longrightarrow> \<Delta> |;| \<Gamma> \<turnstile> t1 as A |:| A" |
   has_type_Let:
-    "\<Gamma> \<turnstile> t1 |:| A \<Longrightarrow> (replace x A \<Gamma>) \<turnstile> t2 |:| B \<Longrightarrow> \<Gamma> \<turnstile> Let var x := t1 in t2 |:| B" |
+    "\<Delta> |;| \<Gamma> \<turnstile> t1 |:| A \<Longrightarrow> \<Delta> |;| (replace x A \<Gamma>) \<turnstile> t2 |:| B \<Longrightarrow> \<Delta> |;| \<Gamma> \<turnstile> Let var x := t1 in t2 |:| B" |
   has_type_Pair:
-    "\<Gamma> \<turnstile> t1 |:| A \<Longrightarrow> \<Gamma> \<turnstile> t2 |:| B \<Longrightarrow> \<Gamma> \<turnstile> \<lbrace>t1,t2\<rbrace> |:| A |\<times>| B" |
+    "\<Delta> |;| \<Gamma> \<turnstile> t1 |:| A \<Longrightarrow> \<Delta> |;| \<Gamma> \<turnstile> t2 |:| B \<Longrightarrow> \<Delta> |;| \<Gamma> \<turnstile> \<lbrace>t1,t2\<rbrace> |:| A |\<times>| B" |
   has_type_Proj1:
-    "\<Gamma> \<turnstile> t1 |:| A |\<times>| B \<Longrightarrow> \<Gamma> \<turnstile> \<pi>1 t1 |:| A" |
+    "\<Delta> |;| \<Gamma> \<turnstile> t1 |:| A |\<times>| B \<Longrightarrow> \<Delta> |;| \<Gamma> \<turnstile> \<pi>1 t1 |:| A" |
   has_type_Proj2:
-    "\<Gamma> \<turnstile> t1 |:| A |\<times>| B \<Longrightarrow> \<Gamma> \<turnstile> \<pi>2 t1 |:| B" |
+    "\<Delta> |;| \<Gamma> \<turnstile> t1 |:| A |\<times>| B \<Longrightarrow> \<Delta> |;| \<Gamma> \<turnstile> \<pi>2 t1 |:| B" |
   has_type_Tuple:
-    "length L = length TL \<Longrightarrow> (\<And>i. 0\<le>i \<Longrightarrow> i< length L \<Longrightarrow> \<Gamma> \<turnstile> (L ! i) |:| (TL ! i))
-      \<Longrightarrow> \<Gamma> \<turnstile> Tuple L |:| \<lparr>TL\<rparr>" |
-  has_type_Proj:
-    "1\<le>i \<Longrightarrow> i\<le> length TL \<Longrightarrow> \<Gamma> \<turnstile> t |:| \<lparr>TL\<rparr> \<Longrightarrow> \<Gamma> \<turnstile> (\<Pi> i t) |:| (TL ! (i-1))"
+    "length L = length TL \<Longrightarrow> (\<And>i. 0\<le>i \<Longrightarrow> i< length L \<Longrightarrow> \<Delta> |;| \<Gamma> \<turnstile> (L ! i) |:| (TL ! i))
+      \<Longrightarrow> \<Delta> |;| \<Gamma> \<turnstile> Tuple L |:| \<lparr>TL\<rparr>" |
+  has_type_ProjT:
+    "1\<le>i \<Longrightarrow> i\<le> length TL \<Longrightarrow> \<Delta> |;| \<Gamma> \<turnstile> t |:| \<lparr>TL\<rparr> \<Longrightarrow> \<Delta> |;| \<Gamma> \<turnstile> (\<Pi> i t) |:| (TL ! (i-1))" |
+  has_type_RCD:
+    "distinct L \<Longrightarrow> length LT = length TL \<Longrightarrow> length L = length LT \<Longrightarrow> (\<And>i. i< length LT \<Longrightarrow> \<Delta> |;| \<Gamma> \<turnstile> (LT ! i) |:| (TL ! i))
+      \<Longrightarrow> \<Delta> |;| \<Gamma> \<turnstile> Record L LT |:| \<lparr>L|:|TL\<rparr>" |
+  has_type_ProjR:
+    "distinct L1 \<Longrightarrow> l\<in> set L1  \<Longrightarrow> length L1 = length TL \<Longrightarrow> \<Delta> |;| \<Gamma> \<turnstile> t |:| \<lparr>L1|:|TL\<rparr> \<Longrightarrow> \<Delta> |;| \<Gamma> \<turnstile> (ProjR l t) |:| (TL ! index L1 l)" |
+  has_type_PatternVar:
+    "coherent_Subst \<Delta> \<Longrightarrow> (k,A)\<in> set \<Delta> \<Longrightarrow> \<Delta> |;| \<Gamma> \<turnstile> (<|V k|>) |:| A" |
+  has_type_PatternRCD:
+    "distinct L \<Longrightarrow> length PL = length TL \<Longrightarrow> length L = length PL \<Longrightarrow> (\<And>i. i< length PL \<Longrightarrow> \<Delta> |;| \<Gamma> \<turnstile> (<|PL ! i|>) |:| (TL ! i))
+      \<Longrightarrow> \<Delta> |;| \<Gamma> \<turnstile> (<|RCD L PL|>) |:| \<lparr>L|:|TL\<rparr>" |
+  has_type_LetNoPattern:
+    "\<Delta> |;| \<Gamma> \<turnstile> t2 |:| A  \<Longrightarrow> \<Delta> |;| \<Gamma> \<turnstile> (Let pattern p := t1 in t2) |:| A" |
+  has_type_LetPattern:
+    "coherent p \<Longrightarrow> Lmatch p t1 \<delta> \<Longrightarrow> length TL = length \<delta> \<Longrightarrow>(\<And>i. i<length TL \<Longrightarrow> \<Delta> |;| \<Gamma> \<turnstile> (snd (\<delta>!i)) |:| (TL!i)) \<Longrightarrow>
+     (zip (fst_extract \<delta>) TL) |;| \<Gamma> \<turnstile> t2 |:| A \<Longrightarrow> \<Delta> |;| \<Gamma> \<turnstile> (Let pattern p := t1 in t2) |:| A" 
+
+
+inductive_cases has_type_LetE : "\<Delta> |;| \<Gamma> \<turnstile> Let var x := t1 in t2 |:| B"
+inductive_cases has_type_ProjTE: "\<Delta> |;| \<Gamma> \<turnstile> \<Pi> i t |:| R"
+inductive_cases has_type_ProjRE: "\<Delta> |;| \<Gamma> \<turnstile> ProjR l t |:| R"
+
   
-inductive_cases has_type_LetE : "\<Gamma> \<turnstile> Let var x := t1 in t2 |:| B"
-inductive_cases has_type_ProjTE: "\<Gamma> \<turnstile> \<Pi> i t |:| R"
+lemma coherent_imp_distinct: "coherent_Subst L \<Longrightarrow> distinct L" 
+by(induction L) (metis distinct_zipI1 zip_comp)+
+  
+lemma coherent_Subst_char: 
+  "coherent_Subst L \<Longrightarrow> p \<in> set L \<Longrightarrow> (\<And>p1. p1\<in> set L-{p} \<Longrightarrow>  fst p \<noteq> fst p1)"
+proof (induction L arbitrary:p)
+  case (Cons a L')
+    from this(2) have 1:"coherent_Subst L' \<and> a \<notin> set L'" 
+      using coherent_imp_distinct
+        by fastforce
+    hence 2:"p=a \<Longrightarrow> fst p \<noteq> fst p1"
+        by (metis Cons(2,4) zip_comp[of L'] Diff_insert_absorb distinct.simps(2) 
+                  list.simps(15) list_iter.simps(2) prod.collapse set_zip_leftD)
+    have "p\<noteq>a \<Longrightarrow> fst p \<noteq> fst p1"
+      proof (cases "p1=a")
+        case False
+          note hyps=this
+          assume H: "p\<noteq>a"
+          with hyps Cons(1,4,3) 1 
+            show ?thesis by auto
+      next
+        case True
+          note hyps =this
+          assume H: "p\<noteq>a"
+          with hyps 
+            show ?thesis
+              proof -
+                have "distinct (fst p1 # fst_extract L')"
+                  using Cons.prems(1) hyps by auto
+                then show ?thesis
+                  by (metis (no_types) Cons.prems(2) H distinct.simps(2) prod.collapse set_ConsD set_zip_leftD zip_comp)
+              qed
+      qed              
+    with 2 show ?case by auto
+qed auto    
+           
+      
+lemma coherent_imp_unique_index:
+  "coherent_Subst L \<Longrightarrow> (n,A) \<in> set L \<Longrightarrow>find (\<lambda>p. fst p = n) L = Some (n,A)"
+proof (induction L)
+  case (Cons a L')
+    have f1: "distinct (fst a # fst_extract L')"
+      using Cons.prems(1) by auto
+    { 
+      assume "a \<noteq> (n, A)"
+      then have "fst a \<noteq> n"
+        by (metis (no_types) Cons.prems(2) Diff_insert_absorb Set.set_insert coherent_Subst_char[OF Cons(2,3)] fst_conv insertE list.set_intros(1))
+      then have "find (\<lambda>p. fst p = n) (a # L') = Some (n, A) \<or> (n, A) = a"
+        using f1 Cons.IH Cons.prems(2) by auto 
+    }
+    thus ?case
+      by fastforce            
+qed auto
 
 lemma inversion:
-  "\<Gamma> \<turnstile> LTrue |:| R \<Longrightarrow> R = Bool"
-  "\<Gamma> \<turnstile> LFalse |:| R \<Longrightarrow> R = Bool"
-  "\<Gamma> \<turnstile> LIf t1 t2 t3 |:| R \<Longrightarrow> \<Gamma> \<turnstile> t1 |:| Bool \<and> \<Gamma> \<turnstile> t2 |:| R \<and> \<Gamma> \<turnstile> t3 |:| R"
-  "\<Gamma> \<turnstile> LVar x |:| R \<Longrightarrow> (x, R) |\<in>| \<Gamma>"
-  "\<Gamma> \<turnstile> LAbs T1 t2 |:| R \<Longrightarrow> \<exists>R2. R = T1 \<rightarrow> R2 \<and> \<Gamma> |,| T1 \<turnstile> t2 |:| R2"
-  "\<Gamma> \<turnstile> LApp t1 t2 |:| R \<Longrightarrow> \<exists>T11. \<Gamma> \<turnstile> t1 |:| T11 \<rightarrow> R \<and> \<Gamma> \<turnstile> t2 |:| T11"
-  "\<Gamma> \<turnstile> unit |:| R \<Longrightarrow> R = Unit"
-  "\<Gamma> \<turnstile> Seq t1 t2 |:| R \<Longrightarrow> \<exists>A. R = A \<and> \<Gamma> \<turnstile> t2 |:| A \<and> \<Gamma> \<turnstile> t1 |:| Unit"
-  "\<Gamma> \<turnstile> t as A |:| R \<Longrightarrow> R = A"
-  "\<Gamma> \<turnstile> Let var x := t in t1 |:| R \<Longrightarrow> \<exists>A B. R = B \<and> \<Gamma> \<turnstile> t |:| A \<and> (replace x A \<Gamma>) \<turnstile> t1 |:| B"
-  "\<Gamma> \<turnstile> \<lbrace>t1,t2\<rbrace> |:| R \<Longrightarrow> \<exists>A B. \<Gamma> \<turnstile> t1 |:| A \<and> \<Gamma> \<turnstile> t2 |:| B \<and> R = A |\<times>| B"
-  "\<Gamma> \<turnstile> \<pi>1 t |:| R \<Longrightarrow> \<exists>A B. \<Gamma> \<turnstile> t |:| A |\<times>| B \<and> R = A"
-  "\<Gamma> \<turnstile> \<pi>2 t |:| R \<Longrightarrow> \<exists>A B. \<Gamma> \<turnstile> t |:| A |\<times>| B \<and> R = B"
-  "\<Gamma> \<turnstile> Tuple L |:| R \<Longrightarrow> \<exists>TL. length L = length TL \<and> (\<forall>i. 0\<le>i \<longrightarrow> i< length L \<longrightarrow> \<Gamma> \<turnstile> (L ! i) |:| (TL ! i)) \<and> R = \<lparr>TL\<rparr>"
-  "\<Gamma> \<turnstile> (\<Pi> i t) |:| R \<Longrightarrow> \<exists>TL. R = (TL ! (i-1)) \<and> \<Gamma> \<turnstile> t |:| \<lparr>TL\<rparr> \<and> 1\<le>i \<and> i\<le> length TL"
+  "\<Delta> |;| \<Gamma> \<turnstile> LTrue |:| R \<Longrightarrow> R = Bool"
+  "\<Delta> |;| \<Gamma> \<turnstile> LFalse |:| R \<Longrightarrow> R = Bool"
+  "\<Delta> |;| \<Gamma> \<turnstile> LIf t1 t2 t3 |:| R \<Longrightarrow> \<Delta> |;| \<Gamma> \<turnstile> t1 |:| Bool \<and> \<Delta> |;| \<Gamma> \<turnstile> t2 |:| R \<and> \<Delta> |;| \<Gamma> \<turnstile> t3 |:| R"
+  "\<Delta> |;| \<Gamma> \<turnstile> LVar x |:| R \<Longrightarrow> (x, R) |\<in>| \<Gamma>"
+  "\<Delta> |;| \<Gamma> \<turnstile> LAbs T1 t2 |:| R \<Longrightarrow> \<exists>R2. R = T1 \<rightarrow> R2 \<and> \<Delta> |;| \<Gamma> |,| T1 \<turnstile> t2 |:| R2"
+  "\<Delta> |;| \<Gamma> \<turnstile> LApp t1 t2 |:| R \<Longrightarrow> \<exists>T11. \<Delta> |;| \<Gamma> \<turnstile> t1 |:| T11 \<rightarrow> R \<and> \<Delta> |;| \<Gamma> \<turnstile> t2 |:| T11"
+  "\<Delta> |;| \<Gamma> \<turnstile> unit |:| R \<Longrightarrow> R = Unit"
+  "\<Delta> |;| \<Gamma> \<turnstile> Seq t1 t2 |:| R \<Longrightarrow> \<exists>A. R = A \<and> \<Delta> |;| \<Gamma> \<turnstile> t2 |:| A \<and> \<Delta> |;| \<Gamma> \<turnstile> t1 |:| Unit"
+  "\<Delta> |;| \<Gamma> \<turnstile> t as A |:| R \<Longrightarrow> R = A"
+  "\<Delta> |;| \<Gamma> \<turnstile> Let var x := t in t1 |:| R \<Longrightarrow> \<exists>A B. R = B \<and> \<Delta> |;| \<Gamma> \<turnstile> t |:| A \<and> \<Delta> |;| (replace x A \<Gamma>) \<turnstile> t1 |:| B"
+  "\<Delta> |;| \<Gamma> \<turnstile> \<lbrace>t1,t2\<rbrace> |:| R \<Longrightarrow> \<exists>A B. \<Delta> |;| \<Gamma> \<turnstile> t1 |:| A \<and> \<Delta> |;| \<Gamma> \<turnstile> t2 |:| B \<and> R = A |\<times>| B"
+  "\<Delta> |;| \<Gamma> \<turnstile> \<pi>1 t |:| R \<Longrightarrow> \<exists>A B. \<Delta> |;| \<Gamma> \<turnstile> t |:| A |\<times>| B \<and> R = A"
+  "\<Delta> |;| \<Gamma> \<turnstile> \<pi>2 t |:| R \<Longrightarrow> \<exists>A B. \<Delta> |;| \<Gamma> \<turnstile> t |:| A |\<times>| B \<and> R = B"
+  "\<Delta> |;| \<Gamma> \<turnstile> Tuple L |:| R \<Longrightarrow> \<exists>TL. length L = length TL \<and> (\<forall>i. 0\<le>i \<longrightarrow> i< length L \<longrightarrow> \<Delta> |;| \<Gamma> \<turnstile> (L ! i) |:| (TL ! i)) \<and> R = \<lparr>TL\<rparr>"
+  "\<Delta> |;| \<Gamma> \<turnstile> (\<Pi> i t) |:| R \<Longrightarrow> \<exists>TL. R = (TL ! (i-1)) \<and> \<Delta> |;| \<Gamma> \<turnstile> t |:| \<lparr>TL\<rparr> \<and> 1\<le>i \<and> i\<le> length TL"
+  "\<Delta> |;| \<Gamma> \<turnstile> (Record L1 LT) |:| R \<Longrightarrow> \<exists>TL. R = \<lparr>L1|:|TL\<rparr> \<and> length TL = length LT \<and> length L1 = length LT \<and> distinct L1 \<and> 
+                                    (\<forall>i. 0\<le>i \<longrightarrow> i< length LT \<longrightarrow> \<Delta> |;| \<Gamma> \<turnstile> (LT ! i) |:| (TL ! i)) " 
+  "\<Delta> |;| \<Gamma> \<turnstile> (ProjR l t) |:| R \<Longrightarrow>\<exists>A m L TL. R = A \<and> \<Delta> |;| \<Gamma> \<turnstile> t |:| \<lparr>L|:|TL\<rparr> \<and> index L l = m \<and> TL ! m = A \<and> distinct L \<and> length L = length TL
+                              \<and> l \<in> set L"
 proof (auto elim: has_type_L.cases has_type_ProjTE)
-  assume H:"\<Gamma> \<turnstile> Let var x := t in t1 |:| R"
-  show "\<exists>A. (length \<Gamma> \<le> x \<longrightarrow> \<Gamma> \<turnstile> t |:| A \<and> \<Gamma> \<turnstile> t1 |:| R) \<and> (\<not> length \<Gamma> \<le> x \<longrightarrow> \<Gamma> \<turnstile> t |:| A \<and> (take x \<Gamma> @ drop (Suc x) \<Gamma> |,| A) \<turnstile> t1 |:| R)"
+  assume H:"\<Delta> |;| \<Gamma> \<turnstile> Let var x := t in t1 |:| R"
+  show "\<exists>A. (length \<Gamma> \<le> x \<longrightarrow> \<Delta> |;| \<Gamma> \<turnstile> t |:| A \<and> \<Delta> |;| \<Gamma> \<turnstile> t1 |:| R) \<and> (\<not> length \<Gamma> \<le> x \<longrightarrow> \<Delta> |;| \<Gamma> \<turnstile> t |:| A \<and> \<Delta> |;| (take x \<Gamma> @ drop (Suc x) \<Gamma> |,| A) \<turnstile> t1 |:| R)"
     using H has_type_LetE
-    by (cases "x\<ge> length \<Gamma>", fastforce+)    
-qed
+    by (cases "x\<ge> length \<Gamma>", fastforce+)
+qed (metis has_type_ProjRE)
 
 lemma canonical_forms:
-  "is_value_L v \<Longrightarrow> \<Gamma> \<turnstile> v |:| Bool \<Longrightarrow> v = LTrue \<or> v = LFalse"
-  "is_value_L v \<Longrightarrow> \<Gamma> \<turnstile> v |:| T1 \<rightarrow> T2 \<Longrightarrow> \<exists>t. v = LAbs T1 t"
-  "is_value_L v \<Longrightarrow> \<Gamma> \<turnstile> v |:| Unit \<Longrightarrow> v = unit"
-  "is_value_L v \<Longrightarrow> \<Gamma> \<turnstile> v |:| A |\<times>| B \<Longrightarrow> \<exists>v1 v2. is_value_L v1 \<and> is_value_L v2 \<and> v= \<lbrace>v1,v2\<rbrace>"
-  "is_value_L v \<Longrightarrow> \<Gamma> \<turnstile> v |:| \<lparr>TL\<rparr> \<Longrightarrow> \<exists>L. is_value_L (Tuple L) \<and> v = Tuple L"
+  "is_value_L v \<Longrightarrow> \<Delta> |;| \<Gamma> \<turnstile> v |:| Bool \<Longrightarrow> v = LTrue \<or> v = LFalse"
+  "is_value_L v \<Longrightarrow> \<Delta> |;| \<Gamma> \<turnstile> v |:| T1 \<rightarrow> T2 \<Longrightarrow> \<exists>t. v = LAbs T1 t"
+  "is_value_L v \<Longrightarrow> \<Delta> |;| \<Gamma> \<turnstile> v |:| Unit \<Longrightarrow> v = unit"
+  "is_value_L v \<Longrightarrow> \<Delta> |;| \<Gamma> \<turnstile> v |:| A |\<times>| B \<Longrightarrow> \<exists>v1 v2. is_value_L v1 \<and> is_value_L v2 \<and> v= \<lbrace>v1,v2\<rbrace>"
+  "is_value_L v \<Longrightarrow> \<Delta> |;| \<Gamma> \<turnstile> v |:| \<lparr>TL\<rparr> \<Longrightarrow> \<exists>L. is_value_L (Tuple L) \<and> v = Tuple L"
+  "is_value_L v \<Longrightarrow> \<Delta> |;| \<Gamma> \<turnstile> v |:| \<lparr>L|:|TL\<rparr> \<Longrightarrow> \<exists>L LT. is_value_L (Record L LT) \<and> v = (Record L LT)" 
 by (auto elim: has_type_L.cases is_value_L.cases)
 
 lemma[simp]: "nat (int x + 1) = Suc x" by simp
@@ -290,41 +454,119 @@ proof -
         by (simp add: drop_Cons' drop_take take_Cons')
     qed
 qed      
-    
-  
+      
 lemma weakening:
-  "\<Gamma> \<turnstile> t |:| A \<Longrightarrow> n \<le> length \<Gamma> \<Longrightarrow> insert_nth n S \<Gamma> \<turnstile> shift_L 1 n t |:| A"
-proof (induction \<Gamma> t A arbitrary: n rule: has_type_L.induct)
-  case (has_type_LAbs \<Gamma> T1 t2 T2)
+  "\<Delta> |;| \<Gamma> \<turnstile> t |:| A \<Longrightarrow> n \<le> length \<Gamma> \<Longrightarrow> \<Delta> |;| insert_nth n S \<Gamma> \<turnstile> shift_L 1 n t |:| A"
+proof (induction \<Delta> \<Gamma> t A arbitrary: n rule: has_type_L.induct)
+  case (has_type_LAbs \<Delta> \<Gamma> T1 t2 T2)
     from has_type_LAbs.prems has_type_LAbs.hyps
       has_type_LAbs.IH[where n="Suc n"] show ?case
       by (auto intro: has_type_L.intros(5))
 next
-  case (has_type_Let \<Gamma> t A x t1 B)
+  case (has_type_Let \<Delta> \<Gamma> t A x t1 B)
     show ?case 
       proof (cases "x\<ge> n")
         assume H:"x\<ge>n"
-        have 1:"insert_nth n S \<Gamma> \<turnstile> shift_L 1 n t |:| A"
+        have 1:"\<Delta> |;| insert_nth n S \<Gamma> \<turnstile> shift_L 1 n t |:| A"
           using has_type_Let(3)[OF has_type_Let(5)]
           by blast
    
-        have "(replace (Suc x) A (insert_nth n S \<Gamma>)) \<turnstile> shift_L 1 n t1 |:| B"
+        have "\<Delta> |;| (replace (Suc x) A (insert_nth n S \<Gamma>)) \<turnstile> shift_L 1 n t1 |:| B"
           using has_type_Let(4,5) H 
                 rep_ins[of n x \<Gamma> S A,OF H has_type_Let(5)]
                 replace_inv_length[of x A \<Gamma>]
           by metis
-        with 1 show "insert_nth n S \<Gamma> \<turnstile> shift_L 1 n (Let var x := t in t1) |:| B"
+        with 1 show "\<Delta> |;| insert_nth n S \<Gamma> \<turnstile> shift_L 1 n (Let var x := t in t1) |:| B"
           using "has_type_L.intros"(10) H
           by auto
       next
         assume H: "\<not> n \<le> x"
-        have a:"replace x A (take n \<Gamma> @ drop n \<Gamma> |,| S) \<turnstile> shift_L 1 n t1 |:| B"
+        have a:"\<Delta> |;| replace x A (take n \<Gamma> @ drop n \<Gamma> |,| S) \<turnstile> shift_L 1 n t1 |:| B"
           using has_type_Let(4)[of n] has_type_Let(5) H
                 rep_ins2[of x n \<Gamma> S A]
                 replace_inv_length[of n A \<Gamma>]
           by simp
-        show "insert_nth n S \<Gamma> \<turnstile> shift_L 1 n (Let var x := t in t1) |:| B"
+        show "\<Delta> |;| insert_nth n S \<Gamma> \<turnstile> shift_L 1 n (Let var x := t in t1) |:| B"
           using has_type_Let(3,5) 
           by (simp add: H, auto intro: a  "has_type_L.intros"(10) )
       qed    
+next
+  case (has_type_ProjT i TL \<Delta> \<Gamma> t)
+    show ?case
+      using "has_type_L.intros"(15)[OF "has_type_ProjT"(1,2)]
+            "has_type_ProjT"(4)[OF "has_type_ProjT"(5)]
+      by force
+next
+  case (has_type_LetPattern p t1 \<delta> TL \<Delta> \<Gamma> t2 A)
+    thus ?case sorry
 qed (auto simp: nth_append min_def intro: has_type_L.intros)
+
+lemma weakening1: "\<Delta> |;| \<Gamma> \<turnstile> t |:| A \<Longrightarrow> (\<exists>P. \<Gamma>' = P @ \<Gamma>) \<Longrightarrow> \<Delta> |;| \<Gamma>' \<turnstile> t |:| A" 
+sorry
+
+lemma has_type_filled:
+  fixes TL::"ltype list" and \<delta>::"(nat\<times>lterm) list" and t::lterm and A::ltype
+  assumes coherentTL: "length TL = length \<delta>" "(\<And>i. i<length TL \<Longrightarrow> \<Delta> |;| \<Gamma> \<turnstile> (snd (\<delta>!i)) |:| (TL!i))"
+           and well_typed_t: "(zip (fst_extract \<delta>) TL) |;| \<Gamma> \<turnstile> t |:| A"
+  shows  "\<Delta> |;| \<Gamma> \<turnstile> fill \<delta> t |:| A"
+using assms(3,1,2)
+proof(induction "(zip (fst_extract \<delta>) TL)" "\<Gamma>" "t" "A" rule: has_type_L.induct)
+  case (has_type_LAbs \<Gamma> T1 t T2)
+    have "\<Delta>|;|\<Gamma> |,| T1 \<turnstile> fill \<delta> t |:| T2"
+      using has_type_LAbs(2)[OF has_type_LAbs(3)]
+            has_type_LAbs(4) weakening1
+      by force            
+    thus ?case
+      by (auto intro: has_type_L.intros(5))
+next
+  case (has_type_Let \<Gamma> t1 A x t2 B)
+    show ?case
+    apply simp
+    apply rule
+    using has_type_Let(2)[OF has_type_Let(5,6)]
+    apply simp
+    using has_type_Let(4)[OF has_type_Let(5)]
+          has_type_Let(3)
+sorry
+next
+  case (has_type_ProjT i TL \<Gamma> t)
+    show ?case
+      using  has_type_L.intros(15)[OF has_type_ProjT(1,2),of \<Delta> \<Gamma> "fill \<delta> t"]
+            has_type_ProjT(4,5,6)
+      by auto
+next
+  case (has_type_PatternVar k A \<Gamma>)
+    hence dist_fst:"distinct (fst_extract \<delta>)"
+      using coherent_imp_distinct
+            fst_extract_zip1 len_fst_extract[of \<delta>]
+      by metis      
+    obtain j where H:"j<length (zip (fst_extract \<delta>) TL) \<and> (zip (fst_extract \<delta>) TL) ! j = (k,A)"
+      using coherent_imp_unique_index[OF "has_type_PatternVar.hyps"]
+            find_Some_iff[of "\<lambda>p. fst p = k" "(zip (fst_extract \<delta>) TL)"]
+      by metis
+    hence "\<Delta>|;|\<Gamma> \<turnstile> snd (\<delta> ! j) |:| (TL ! j)"       
+      using "has_type_PatternVar"(3,4) 
+      by simp
+    with H show ?case       
+      using coherent_imp_unique_index[OF "has_type_PatternVar.hyps"]
+            zip_comp[of \<delta>]
+            dist_fst
+            "has_type_PatternVar"(3)
+            find_zip1[OF dist_fst, of TL "snd_extract \<delta>" j k]
+            len_fst_extract[of \<delta>] len_snd_extract[of \<delta>]
+    by force
+next
+  case (has_type_LetPattern p t1 \<delta>1 TL \<Gamma> t2 A)
+    show ?case
+      apply simp
+      apply rule
+      apply(simp add: has_type_LetPattern(1))
+      prefer 2
+      using has_type_LetPattern(3)
+      apply auto[1]
+      prefer 2
+      using has_type_LetPattern
+
+    sorry
+qed (auto intro:has_type_L.intros)
+
